theories/Template/QuoteGround.v
@@ -1,0 +1,192 @@
+From MetaCoq.Template Require Import Ast utils All.
+From MetaCoq.Lob.Template Require Import
+     QuoteGround.Init QuoteGround.Init.Typing
+     QuoteGround.Ast QuoteGround.Typing
+     QuoteGround.Ast.Typing QuoteGround.Typing.Typing
+     QuoteGround.Typed
+.
+From MetaCoq.Lob Require Import Template.Typed.
+
+(* Does the env contain everything necessary for quoting? *)
+Axiom env_can_quote : Typed.env -> bool.
+Record env := { env_ :> Typed.env ; env_good : env_can_quote env_ }.
+Existing Class env.
+#[export] Existing Instance env_.
+
+Local Ltac use_well_typed _ :=
+  let qwt := lazymatch goal with
+             | [ |- _ ;;; _ |- @quote_ground ?T ?quoteT ?t : _ ]
+               => constr:(ltac:(notypeclasses refine (_ : @ground_quotable_well_typed _ T _ quoteT); typeclasses eauto))
+             | [ |- _ ;;; _ |- ?q : _ ]
+               => constr:(ltac:(notypeclasses refine (_ : @quotation_of_well_typed _ _ _ _ q); typeclasses eauto))
+             end in
+  first [ eapply qwt
+        | eapply type_Conv; [ eapply qwt | repeat exactly_once constructor .. ] ];
+  try apply context_wf_local; auto; try exact eq_refl;
+  cbv [config.global_env_ext_constraint]; cbn [fold_right map].
+
+(* For now, let's assume a rigid environment tiled at all levels.  TODO: Think about weakening *)
+(*
+Axiom env_subset : env -> env -> bool.
+(* copy ⊂_cs level *)
+Infix "⊂_e" := env_subset (at level 30).
+ *)
+Axiom proof_admitted : False.
+Section in_env.
+  Context {Σ : env}.
+  (* the universe that can contain all the quoted things *)
+  Definition u : sort.
+  Proof using Σ.
+    unshelve econstructor.
+    { refine (Universe.lType _).
+      abstract case proof_admitted. }
+    { abstract (case proof_admitted) using wf_u. }
+  Defined.
+
+  #[local] Hint Resolve wf_u : core.
+
+  (* We assume we're quoting to a fixed context *)
+  Section in_context.
+    Context {Γ : context}.
+    Local Ltac do_admit _ :=
+      let G := lazymatch goal with |- ?G => G end in
+      try (assert_fails has_evar G;
+           lazymatch G with context[Σ] => idtac end;
+           lazymatch G with
+           | is_true _ => idtac
+           | compare_universe _ _ _ _ => idtac
+           end;
+           abstract case proof_admitted).
+    Local Ltac use_well_typed_then_admit _ :=
+      use_well_typed ();
+      do_admit ().
+    Local Ltac misc _ :=
+      lazymatch goal with
+      | [ |- _ = false ] => vm_compute; reflexivity
+      | [ |- _ <> _ ] => congruence
+      | _ => idtac
+      end.
+
+    #[local] Obligation Tactic := intros; try use_well_typed_then_admit ().
+
+    #[program] Definition qenv : type Γ u
+      := {| type_ := Typed.qenv |}.
+    #[program] Definition qΣ : term (Γ:=Γ) qenv
+      := {| term_ := quote_ground Σ.(env_) |}.
+    #[program] Definition qcontext : type Γ u
+      := {| type_ := _ : quotation_of (@Typed.context Σ) |}.
+    Next Obligation.
+      econstructor; try use_well_typed_then_admit (); misc ().
+      repeat exactly_once econstructor; try use_well_typed_then_admit (); misc ().
+      econstructor.
+      try use_well_typed_then_admit ().
+      2: econstructor.
+      all: repeat repeat exactly_once econstructor; do_admit ().
+      econstructor.
+      all: repeat repeat exactly_once constructor; try apply context_wf_local; auto.
+      hnf; econstructor.
+      use_well_typed_then_admit ().
+      abstract case proof_admitted.
+    Qed.
+    #[program] Definition qsort : type Γ u
+      := {| type_ := _ : quotation_of (@Typed.sort Σ) |}.
+    Next Obligation.
+      econstructor; try use_well_typed_then_admit (); misc ().
+      repeat exactly_once econstructor; try use_well_typed_then_admit (); misc ().
+      econstructor.
+      try use_well_typed_then_admit ().
+      2: econstructor.
+      all: repeat repeat exactly_once econstructor; do_admit ().
+      econstructor.
+      all: repeat repeat exactly_once constructor; try apply context_wf_local; auto.
+      hnf; econstructor.
+      use_well_typed_then_admit ().
+      abstract case proof_admitted.
+    Admitted.
+    #[program] Definition qtype (qΓ' : term qcontext) (qs : term qsort) : type Γ u
+      := {| type_ := tApp <% @Typed.type %> [qΣ:Ast.term; qΓ':Ast.term; qs:Ast.term] |}.
+    Next Obligation.
+      econstructor; try use_well_typed_then_admit (); misc ().
+      econstructor; try apply qΣ.
+      all: econstructor.
+      all: do 4 lazymatch goal with
+                | [ |- _ ;;; _ |- (@type_ _ _ _ ?q) : _ ] => apply q
+                | [ |- _ ;;; _ |- (@term_ _ _ _ _ ?q) : _ ] => apply q
+                | [ |- _ ;;; _ |- tProd _ _ _ : tSort _ ] => econstructor
+                | [ |- _ ;;; _ |- tApp _ _ : tSort _ ] => econstructor
+                | [ |- _ ;;; _ |- tProd _ _ _ <= tProd _ _ _ ] => econstructor
+                | _ => try exactly_once econstructor; cbn [subst1 subst0]
+                end.
+      all: try misc ().
+      all: try exactly_once econstructor.
+      all: try exactly_once econstructor.
+      all: try exactly_once econstructor.
+      all: try exactly_once econstructor.
+      all: try exactly_once econstructor.
+      all: try exactly_once econstructor.
+      all: try exactly_once econstructor.
+    Abort.
+    (*
+      all: try exactly_once econstructor.
+      all: try exactly_once econstructor.
+      all: match goal with
+      end.
+goal 7 (ID 796) is:
+ Σ;;; Γ |- tProd ?na' (subst0 [qΣ] ?a') (subst [qΣ] 1 ?b') <= tProd ?na qcontext ?B
+goal 8 (ID 807) is:
+ Σ;;; Γ |- tProd ?na0 qsort ?B0 : tSort ?s0
+goal 9 (ID 813) is:
+ Σ;;; Γ |- ?B {0 := qΓ'} <= tProd ?na0 qsort ?B0
+
+      7: { cbn [subst1 subst0]. Set Printing All. constructor.
+      all:
+      all: lazymatch goal with
+           | [ |- _ ;;; _ |- (@type_ _ _ _ ?q) : _ ] => apply q
+           | [ |- _ ;;; _ |- (@term_ _ _ _ _ ?q) : _ ] => apply q
+           | _ => idtac
+           end.
+
+      all: lazymatch goal with
+           | [ |- _ ;;; _ |- (@type_ _ _ _ ?q) : _ ] => apply q
+           | [ |- _ ;;; _ |- (@term_ _ _ _ _ ?q) : _ ] => apply q
+           | [ |- _ ;;; _ |- (@sort_ _ _ _ _ ?q) : _ ] => apply q
+           | _ => idtac
+           end.
+      eapply qenv.
+
+      all: repeat exactly_once econstructor.
+      econstructor.
+      try use_well_typed_then_admit ().
+      2: econstructor.
+      all: repeat repeat exactly_once econstructor; do_admit ().
+      econstructor.
+      all: repeat repeat exactly_once constructor; try apply context_wf_local; auto.
+      hnf; econstructor.
+      use_well_typed_then_admit ().
+      abstract case proof_admitted.
+    Admitted.
+    #[program] Definition qterm {qΓ' : term qcontext} {qs : term qsort} {qT : term (qtype qΓ' qs)} : type Γ u
+      := {| type_ := tApp <% @Typed.term %> [qΣ:Ast.term; qΓ':Ast.term; qs:Ast.term; qT:Ast.term] |}.
+    Next Obligation.
+    Admitted.
+
+    Definition quote_context (Γ' : context) : term qcontext.
+
+               Definition quote_term {s : sort} {T : type Γ s} (t : term T) : Type.
+  refine (@term Σ _ _ _).
+  :=
+
+Definition quote_env : env
+Local Set Primitive Projections.
+Record env := { env_ :> global_env_ext ; checker_flags_ :> config.checker_flags  }.
+Existing Class env.
+#[export] Existing Instance checker_flags_.
+Record context {Σ : env} := { context_ :> Ast.Env.context }.
+Record sort {Σ : env} := { sort_ :> Universe.t }.
+Record type {Σ : env} (Γ : context) (s : sort) :=
+  { type_ :> Ast.term ; type_well_typed : Σ ;;; Γ |- type_ : tSort s }.
+Record term {s : sort} (T : type Γ s) :=
+  { term_ :> Ast.term ; term_well_typed : Σ ;;; Γ |- term_ : T }.
+
+Definition quote
+*)
