theories/Template/QuoteGround/Ast/Typing.v
@@ -1,0 +1,96 @@
+From MetaCoq.Lob.Template Require Import QuoteGround.Ast.
+From MetaCoq.Lob.Template.QuoteGround Require Export Coq.Init.Typing.
+From MetaCoq.Template Require Import Ast Induction.
+(*
+From MetaCoq.Lob.Template.QuoteGround Require Export utils Environment EnvironmentTyping Universes BasicAst.
+*)
+(*
+#[export] Instance quote_predicate {term} {qterm : quotation_of term} {quote_term : ground_quotable term} : ground_quotable (predicate term) := ltac:(destruct 1; exact _).
+#[export] Instance quote_branch {term} {qterm : quotation_of term} {quote_term : ground_quotable term} : ground_quotable (branch term) := ltac:(destruct 1; exact _).
+#[local] Hint Extern 1 => assumption : typeclass_instances.
+ *)
+#[export] Instance quote_term_well_typed : ground_quotable_well_typed_using [term] term.
+Proof.
+Admitted.
+
+(*
+Module QuoteTemplateTerm <: QuoteTerm TemplateTerm.
+  #[export] Instance qterm : quotation_of TemplateTerm.term := _.
+  #[export] Instance quote_term : ground_quotable TemplateTerm.term := _.
+
+  #[export] Instance qtRel : quotation_of TemplateTerm.tRel := _.
+  #[export] Instance qtSort : quotation_of TemplateTerm.tSort := _.
+  #[export] Instance qtProd : quotation_of TemplateTerm.tProd := _.
+  #[export] Instance qtLambda : quotation_of TemplateTerm.tLambda := _.
+  #[export] Instance qtLetIn : quotation_of TemplateTerm.tLetIn := _.
+  #[export] Instance qtInd : quotation_of TemplateTerm.tInd := _.
+  #[export] Instance qtProj : quotation_of TemplateTerm.tProj := _.
+  #[export] Instance qmkApps : quotation_of TemplateTerm.mkApps := _.
+
+  #[export] Instance qlift : quotation_of TemplateTerm.lift := _.
+  #[export] Instance qsubst : quotation_of TemplateTerm.subst := _.
+  #[export] Instance qclosedn : quotation_of TemplateTerm.closedn := _.
+  #[export] Instance qnoccur_between : quotation_of TemplateTerm.noccur_between := _.
+  #[export] Instance qsubst_instance_constr : quotation_of TemplateTerm.subst_instance_constr := _.
+  Module Instances.
+    #[export] Existing Instances
+     qterm
+     quote_term
+
+     qtRel
+     qtSort
+     qtProd
+     qtLambda
+     qtLetIn
+     qtInd
+     qtProj
+     qmkApps
+
+     qlift
+     qsubst
+     qclosedn
+     qnoccur_between
+     qsubst_instance_constr
+    .
+  End Instances.
+End QuoteTemplateTerm.
+Export QuoteTemplateTerm.Instances.
+
+Module QuotationOfEnv <: QuotationOfEnvironment TemplateTerm Env.
+  #[export] Instance qconstructor_body : inductive_quotation_of constructor_body := _.
+  #[export] Instance qprojection_body : inductive_quotation_of projection_body := _.
+  #[export] Instance qone_inductive_body : inductive_quotation_of one_inductive_body := _.
+  #[export] Instance qmutual_inductive_body : inductive_quotation_of mutual_inductive_body := _.
+  #[export] Instance qconstant_body : inductive_quotation_of constant_body := _.
+  #[export] Instance qglobal_decl : inductive_quotation_of global_decl := _.
+  #[export] Instance qglobal_env : inductive_quotation_of global_env := _.
+  #[export] Instance qAll_decls : inductive_quotation_of All_decls := _.
+  #[export] Instance qAll_decls_alpha : inductive_quotation_of All_decls_alpha := _.
+  Module Instances.
+    #[export] Existing Instances
+     qconstructor_body
+     qprojection_body
+     qone_inductive_body
+     qmutual_inductive_body
+     qconstant_body
+     qglobal_decl
+     qglobal_env
+     qAll_decls
+     qAll_decls_alpha
+    .
+  End Instances.
+End QuotationOfEnv.
+Export QuotationOfEnv.Instances.
+
+Module QuoteEnv := QuoteEnvironment TemplateTerm Env QuoteTemplateTerm QuotationOfEnv.
+Export QuoteEnv.Instances.
+
+Module QuoteTemplateLookup := QuoteLookup TemplateTerm Env TemplateLookup QuoteTemplateTerm QuotationOfEnv.
+Export QuoteTemplateLookup.Instances.
+
+#[export] Instance quote_parameter_entry : ground_quotable parameter_entry := ltac:(destruct 1; exact _).
+#[export] Instance quote_definition_entry : ground_quotable definition_entry := ltac:(destruct 1; exact _).
+#[export] Instance quote_constant_entry : ground_quotable constant_entry := ltac:(destruct 1; exact _).
+#[export] Instance quote_one_inductive_entry : ground_quotable one_inductive_entry := ltac:(destruct 1; exact _).
+#[export] Instance quote_mutual_inductive_entry : ground_quotable mutual_inductive_entry := ltac:(destruct 1; exact _).
+*)
